Coq/safe.v
@@ -10,6 +10,20 @@ Require Import List.
 Require Import CpdtTactics.
 Require Import Coq.Logic.FunctionalExtensionality.
 
+Lemma linked_class :
+  forall M1 M2 M, M1 ⋄ M2 ≜ M ->
+             forall C Def, C <> ObjectName ->
+                      M1 C = Some Def ->
+                      M C = Some Def.
+Proof.
+  intros M1 M2 M Hlink;
+    inversion Hlink;
+    subst;
+    intros;
+    unfold extend;
+    crush.
+Qed.
+
 Lemma substmt_trans :
   forall s2 s3, substmt s2 s3 ->
            forall s1, substmt s1 s2 ->
@@ -75,12 +89,10 @@ Proof.
           inversion H13;
           subst.
         assert (Htmp : o2 =
-                       {|
-                         cname := cname o1;
-                         flds := fun x : fld => if eqb x f then Some v else flds o1 x;
-                         meths := meths o1 |});
+                       {| cname := cname o1;
+                          flds := fun x : fld => if eqb x f then Some v else flds o1 x |});
           [crush|rewrite Htmp in H16; unfold flds in *].
-        assert (Hflds : (let (_, flds, _) := o1 in flds) = (flds o1));
+        assert (Hflds : (let (_, flds) := o1 in flds) = (flds o1));
           [auto|rewrite Hflds in H16].
         eq_auto.
         crush.
@@ -90,12 +102,10 @@ Proof.
           inversion H13;
           subst.
         assert (Htmp : o2 =
-                       {|
-                         cname := cname o1;
-                         flds := fun x : fld => if eqb x f then Some v else flds o1 x;
-                         meths := meths o1 |});
+                       {| cname := cname o1;
+                          flds := fun x : fld => if eqb x f then Some v else flds o1 x |});
           [crush|rewrite Htmp in H16; unfold flds in *].
-        assert (Hflds : (let (_, flds, _) := o1 in flds) = (flds o1));
+        assert (Hflds : (let (_, flds) := o1 in flds) = (flds o1));
           [auto|rewrite Hflds in H16].
         eq_auto.
         crush.
@@ -113,13 +123,13 @@ Qed.
 
 Lemma reductions_prop_change :
   forall M σ1 σ2, reductions M σ1 σ2 ->
-             forall P, ~ P σ1 ->
-                  P σ2 ->
-                  exists σ σ', M ∙ σ ⤳ σ' /\
-                          ~ P σ /\
-                          P σ' /\
-                          (reductions M σ1 σ \/ σ1 = σ) /\
-                          (reductions M σ' σ2 \/ σ2 = σ').
+                  forall P, ~ P σ1 ->
+                            P σ2 ->
+                            exists σ σ', M ∙ σ ⤳ σ' /\
+                                    ~ P σ /\
+                                    P σ' /\
+                                    (reductions M σ1 σ \/ σ1 = σ) /\
+                                    (reductions M σ' σ2 \/ σ2 = σ').
 Proof.
   intros M σ1 σ2 Hred;
     induction Hred;
@@ -136,7 +146,7 @@ Proof.
       match goal with
       | [Ha : reductions ?M ?σ1 ?σ \/ ?σ1 = ?σ,
               Hb : reductions ?M ?σ' ?σ2 \/ ?σ2 = ?σ' |- _] =>
-       destruct Ha, Hb
+        destruct Ha, Hb
       end;
         subst;
         try solve [repeat eexists; eauto with loo_db].
@@ -155,22 +165,22 @@ Inductive stmt_in_method : mdl -> heap -> addr -> mth -> stmt -> Prop :=
                                        substmt s sm ->
                                        stmt_in_method M χ α m s.
 
-Inductive method_is_called : config -> addr -> mth -> partial_map var value -> Prop :=
+Inductive method_is_called : config -> var -> addr -> mth -> partial_map var value -> Prop :=
 | meth_called : forall x y m β s α ϕ χ ψ, contn ϕ = c_stmt (s_meth x y m β ;; s) ->
                                      ⌊ y ⌋ (χ, ϕ :: ψ) ≜ (v_addr α) ->
-                                     method_is_called (χ, ϕ::ψ) α m (β ∘ (vMap ϕ)).
+                                     method_is_called (χ, ϕ::ψ) x α m (β ∘ (vMap ϕ)).
 
 Hint Constructors method_is_called stmt_in_method : loo_db.
 
 Lemma arising_frame_is_method_call_reduction :
   forall M σ1 σ2, M ∙ σ1 ⤳ σ2 ->
-             forall χ1 χ2 ϕ1 ϕ2 ψ1 ψ2,
-               σ1 = (χ1, ϕ1 :: ψ1) ->
-               σ2 = (χ2, ϕ2 :: ψ2) ->
-               length (snd σ1) < length (snd σ2) ->
-               (exists α m β s, method_is_called σ1 α m β /\
-                           contn ϕ2 = c_stmt s /\
-                           stmt_in_method M χ1 α m s).
+                  forall χ1 χ2 ϕ1 ϕ2 ψ1 ψ2,
+                    σ1 = (χ1, ϕ1 :: ψ1) ->
+                    σ2 = (χ2, ϕ2 :: ψ2) ->
+                    length (snd σ1) < length (snd σ2) ->
+                    (exists x α m β s, method_is_called σ1 x α m β /\
+                                  contn ϕ2 = c_stmt s /\
+                                  stmt_in_method M χ1 α m s).
 Proof.
   intros M σ1 σ2 Hred;
     induction Hred;
@@ -179,7 +189,7 @@ Proof.
     crush;
     repeat simpl_crush.
 
-  exists α, m, (ps ∘ vMap ϕ1), s;
+  exists x, α, m, (ps ∘ vMap ϕ1), s;
     repeat split;
     simpl in *;
     eauto with loo_db.
@@ -225,19 +235,19 @@ Qed.*)
 
 Lemma arising_frame_is_method_call_reductions :
   forall M σ1 σ2, reductions M σ1 σ2 ->
-             forall χ1 χ2 ϕ1 ψ2,
-               σ1 = (χ1, ϕ1 :: nil) ->
-               σ2 = (χ2, ψ2) ->
-               forall ϕ2, In ϕ2 ψ2 ->
-                     (exists ψ', ψ2 = ψ' ++ ϕ2 :: nil) \/
-                     (exists α m β s, method_is_called σ1 α m β /\
-                                 contn ϕ2 = c_stmt s /\
-                                 stmt_in_method M χ1 α m s) \/
-                     (exists χ ϕ ψ α m β s, reductions M σ1 (χ, ϕ :: ψ) /\
-                                       reductions M (χ, ϕ :: ψ) σ2 /\
-                                       method_is_called (χ, ϕ :: ψ) α m β /\
-                                       (contn ϕ2 = c_stmt s \/ exists x, contn ϕ2 = c_hole x s) /\
-                                       stmt_in_method M χ α m s).
+                  forall χ1 χ2 ϕ1 ψ2,
+                    σ1 = (χ1, ϕ1 :: nil) ->
+                    σ2 = (χ2, ψ2) ->
+                    forall ϕ2, In ϕ2 ψ2 ->
+                               (exists ψ', ψ2 = ψ' ++ ϕ2 :: nil) \/
+                               (exists x α m β s, method_is_called σ1 x α m β /\
+                                             contn ϕ2 = c_stmt s /\
+                                             stmt_in_method M χ1 α m s) \/
+                               (exists χ ϕ ψ x α m β s, reductions M σ1 (χ, ϕ :: ψ) /\
+                                                   reductions M (χ, ϕ :: ψ) σ2 /\
+                                                   method_is_called (χ, ϕ :: ψ) x α m β /\
+                                                   (contn ϕ2 = c_stmt s \/ exists y, contn ϕ2 = c_hole y s) /\
+                                                   stmt_in_method M χ α m s).
 Proof.
   intros M σ1 σ2 Hred;
     induction Hred;
@@ -281,7 +291,6 @@ Proof.
 
   - admit.
 Admitted.
-               
 
 (*Lemma arising_frame_is_method_call_reductions :
   forall M σ1 σ2, reductions M σ1 σ2 ->
@@ -597,10 +606,10 @@ Qed.*)
 
 Lemma bottom_frame_remains_in_stack_reduction :
   forall M σ1 σ2, M ∙ σ1 ⤳ σ2 ->
-             forall χ1 ϕ1 ψ1,
-               σ1 = (χ1, ψ1 ++ ϕ1 :: nil) ->
-               exists ψ ϕ, (snd σ2) = (ψ ++ ϕ :: nil) /\
-                      vMap ϕ this = vMap ϕ1 this.
+                  forall χ1 ϕ1 ψ1,
+                    σ1 = (χ1, ψ1 ++ ϕ1 :: nil) ->
+                    exists ψ ϕ, (snd σ2) = (ψ ++ ϕ :: nil) /\
+                                vMap ϕ this = vMap ϕ1 this.
 Proof.
   intros M σ1 σ2 Hred;
     induction Hred;
@@ -634,10 +643,10 @@ Qed.
 
 Lemma bottom_frame_remains_in_stack_reductions :
   forall M σ1 σ2, reductions M σ1 σ2 ->
-             forall χ1 ϕ1 ψ1,
-               σ1 = (χ1, ψ1 ++ ϕ1 :: nil) ->
-               exists ψ ϕ, (snd σ2) = (ψ ++ ϕ :: nil) /\
-                      vMap ϕ this = vMap ϕ1 this.
+                  forall χ1 ϕ1 ψ1,
+                    σ1 = (χ1, ψ1 ++ ϕ1 :: nil) ->
+                    exists ψ ϕ, (snd σ2) = (ψ ++ ϕ :: nil) /\
+                                vMap ϕ this = vMap ϕ1 this.
 Proof.
   intros M σ1 σ2 Hred;
     induction Hred;
@@ -649,7 +658,7 @@ Proof.
   - destruct (IHHred χ1 ϕ1 ψ1); auto;
       destruct_exists_loo;
       andDestruct;
-        subst.
+      subst.
 
     destruct σ2 as [χ ψ];
       simpl in *;
@@ -661,13 +670,13 @@ Qed.
 
 Lemma different_this_implies_larger_stack_reductions :
   forall M σ1 σ2, reductions M σ1 σ2 ->
-             σ_wf σ1 ->
-             forall χ1 ϕ1,
-               σ1 = (χ1, ϕ1 :: nil) ->
-               forall v1 v2, ⌊ this ⌋ σ1 ≜ v1 ->
-                        ⌊ this ⌋ σ2 ≜ v2 ->
-                        (length (snd σ1) < length (snd σ2)) \/
-                        (v1 = v2 /\ length (snd σ1) = length (snd σ2)).
+                  σ_wf σ1 ->
+                  forall χ1 ϕ1,
+                    σ1 = (χ1, ϕ1 :: nil) ->
+                    forall v1 v2, ⌊ this ⌋ σ1 ≜ v1 ->
+                                  ⌊ this ⌋ σ2 ≜ v2 ->
+                                  (length (snd σ1) < length (snd σ2)) \/
+                                  (v1 = v2 /\ length (snd σ1) = length (snd σ2)).
 Proof.
   intros.
   destruct (bottom_frame_remains_in_stack_reductions M σ1 σ2 H χ1 ϕ1 nil)
@@ -691,14 +700,7 @@ Proof.
     end;
       simpl in *;
       repeat simpl_crush.
-    match goal with
-    | [ Ha : vMap ?ϕ1 ?x = vMap ?ϕ2 ?x,
-             Hb : vMap ?ϕ1 ?x = Some _,
-                  Hc : vMap ?ϕ2 ?x = Some _ |- _] =>
-      rewrite Ha in Hb;
-        rewrite Hb in Hc
-    end;
-      crush.
+    crush.
 
   - simpl;
       rewrite app_length;
@@ -707,7 +709,7 @@ Qed.
 
 Lemma reduction_implies_non_empty_stack_1 :
   forall M σ1 σ2, M ∙ σ1 ⤳ σ2 ->
-             exists χ1 ϕ1 ψ1, σ1 = (χ1, ϕ1 :: ψ1).
+                  exists χ1 ϕ1 ψ1, σ1 = (χ1, ϕ1 :: ψ1).
 Proof.
   intros M σ1 σ2 Hred;
     induction Hred;
@@ -717,7 +719,7 @@ Qed.
 
 Lemma reduction_implies_non_empty_stack_2 :
   forall M σ1 σ2, M ∙ σ1 ⤳ σ2 ->
-             exists χ2 ϕ2 ψ2, σ2 = (χ2, ϕ2 :: ψ2).
+                  exists χ2 ϕ2 ψ2, σ2 = (χ2, ϕ2 :: ψ2).
 Proof.
   intros M σ1 σ2 Hred;
     induction Hred;
@@ -727,8 +729,8 @@ Qed.
 
 Lemma reduction_preserves_heap_locations :
   forall M σ1 σ2, M ∙ σ1 ⤳ σ2 ->
-             forall α (o : obj), mapp σ1 α = Some o ->
-                            exists o', mapp σ2 α = Some o'.
+                  forall α (o : obj), mapp σ1 α = Some o ->
+                                      exists o', mapp σ2 α = Some o'.
 Proof.
   intros M σ1 σ2 Hred;
     induction Hred;
@@ -746,9 +748,9 @@ Qed.
 
 Lemma reductions_preserves_heap_locations_classes :
   forall M σ1 σ2, reductions M σ1 σ2 ->
-             forall α (o : obj), mapp σ1 α = Some o ->
-                            exists o', mapp σ2 α = Some o' /\
-                                  cname o' = cname o.
+                  forall α (o : obj), mapp σ1 α = Some o ->
+                                      exists o', mapp σ2 α = Some o' /\
+                                                 cname o' = cname o.
 Proof.
   intros M σ1 σ2 Hred;
     induction Hred;
@@ -762,7 +764,7 @@ Proof.
       destruct_exists_loo;
       andDestruct.
     apply reduction_preserves_addr_classes
-            with (α:=α)(o1:=o0) in H;
+      with (α:=α)(o1:=o0) in H;
       eauto;
       repeat destruct_exists_loo;
       andDestruct.
@@ -771,10 +773,10 @@ Qed.
 
 Lemma reduction_preserves_fields :
   forall M σ1 σ2, M ∙ σ1 ⤳ σ2 ->
-             forall α o f v, mapp σ1 α = Some o ->
-                        flds o f = Some v ->
-                        exists o' v', mapp σ2 α = Some o' /\
-                                 flds o' f = Some v'.
+                  forall α o f v, mapp σ1 α = Some o ->
+                                  flds o f = Some v ->
+                                  exists o' v', mapp σ2 α = Some o' /\
+                                                flds o' f = Some v'.
 Proof.
   intros M σ1 σ2 Hred;
     induction Hred;
@@ -821,10 +823,10 @@ Qed.
 
 Lemma reductions_preserves_fields :
   forall M σ1 σ2, reductions M σ1 σ2 ->
-             forall α o f v, mapp σ1 α = Some o ->
-                        flds o f = Some v ->
-                        exists o' v', mapp σ2 α = Some o' /\
-                                 flds o' f = Some v'.
+                  forall α o f v, mapp σ1 α = Some o ->
+                                  flds o f = Some v ->
+                                  exists o' v', mapp σ2 α = Some o' /\
+                                                flds o' f = Some v'.
 Proof.
   intros M σ1 σ2 Hred;
     induction Hred;
@@ -842,21 +844,21 @@ Qed.
 
 Lemma reductions_field_change :
   forall M σ1 σ2, reductions M σ1 σ2 ->
-             forall χ1 ϕ1 ψ1 χ2 ϕ2 ψ2,
-               σ1 = (χ1, ϕ1 :: ψ1) ->
-               σ2 = (χ2, ϕ2 :: ψ2) ->
-               forall α o1 o2 f v1 v2,
-                 mapp σ1 α = Some o1 ->
-                 mapp σ2 α = Some o2 ->
-                 flds o1 f = Some v1 ->
-                 flds o2 f = Some v2 ->
-                 v1 <> v2 ->
-                 exists χ ϕ ψ, (reductions M σ1 (χ, ϕ :: ψ) \/ σ1 = (χ, ϕ :: ψ)) /\
-                          exists  x y s C, contn ϕ = c_stmt ((x ◌ f) ≔ (r_ y) ;; s) /\
-                                      ⌊ x ⌋ (χ, ϕ :: ψ) ≜ (v_addr α) /\
-                                      classOf this (χ, ϕ :: ψ) C /\
-                                      classOf x (χ, ϕ :: ψ) C /\
-                                      ⌊ y ⌋ (χ, ϕ :: ψ) ≜ v2.
+                  forall χ1 ϕ1 ψ1 χ2 ϕ2 ψ2,
+                    σ1 = (χ1, ϕ1 :: ψ1) ->
+                    σ2 = (χ2, ϕ2 :: ψ2) ->
+                    forall α o1 o2 f v1 v2,
+                      mapp σ1 α = Some o1 ->
+                      mapp σ2 α = Some o2 ->
+                      flds o1 f = Some v1 ->
+                      flds o2 f = Some v2 ->
+                      v1 <> v2 ->
+                      exists χ ϕ ψ, (reductions M σ1 (χ, ϕ :: ψ) \/ σ1 = (χ, ϕ :: ψ)) /\
+                                    exists  x y s C, contn ϕ = c_stmt ((x ◌ f) ≔ (r_ y) ;; s) /\
+                                                     ⌊ x ⌋ (χ, ϕ :: ψ) ≜ (v_addr α) /\
+                                                     classOf this (χ, ϕ :: ψ) C /\
+                                                     classOf x (χ, ϕ :: ψ) C /\
+                                                     ⌊ y ⌋ (χ, ϕ :: ψ) ≜ v2.
 Proof.
   intros.
   destruct (reductions_prop_change M σ1 σ2)
@@ -959,17 +961,17 @@ Qed.
 
 Lemma frame_arising_from_single_frame_is_method_call_reductions :
   forall M σ1 σ2, reductions M σ1 σ2 ->
-             forall χ1 ϕ1,
-               σ1 = (χ1, ϕ1 :: nil) ->
-               mapp σ1 this <> mapp σ2 this ->
-               forall χ2 ϕ2 ψ2, σ2 = (χ2, ϕ2 :: ψ2) ->
-                           (exists α m β s, method_is_called σ1 α m β /\
-                                       contn ϕ2 = c_stmt s /\
-                                       stmt_in_method M χ1 α m s) \/
-                           (exists χ ϕ ψ α m β s, reductions M σ1 (χ, ϕ :: ψ) /\
-                                             method_is_called (χ, ϕ :: ψ) α m β /\
-                                             contn ϕ2 = c_stmt s /\
-                                             stmt_in_method M χ α m s).
+                  forall χ1 ϕ1,
+                    σ1 = (χ1, ϕ1 :: nil) ->
+                    mapp σ1 this <> mapp σ2 this ->
+                    forall χ2 ϕ2 ψ2, σ2 = (χ2, ϕ2 :: ψ2) ->
+                                (exists x α m β s, method_is_called σ1 x α m β /\
+                                              contn ϕ2 = c_stmt s /\
+                                              stmt_in_method M χ1 α m s) \/
+                                (exists χ ϕ ψ x α m β s, reductions M σ1 (χ, ϕ :: ψ) /\
+                                                    method_is_called (χ, ϕ :: ψ) x α m β /\
+                                                    contn ϕ2 = c_stmt s /\
+                                                    stmt_in_method M χ α m s).
 Proof.
   intros.
 (*  destruct (arising_frame_is_method_call_reductions M σ1 σ2)
@@ -1000,23 +1002,23 @@ Admitted.
 
 Lemma reductions_field_change_not_this :
   forall M σ1 σ2, reductions M σ1 σ2 ->
-             forall χ1 ϕ1 ψ1 χ2 ϕ2 ψ2,
-               σ1 = (χ1, ϕ1 :: ψ1) ->
-               σ2 = (χ2, ϕ2 :: ψ2) ->
-               forall α o1 o2 f v1 v2,
-                 mapp σ1 α = Some o1 ->
-                 mapp σ2 α = Some o2 ->
-                 flds o1 f = Some v1 ->
-                 flds o2 f = Some v2 ->
-                 v1 <> v2 ->
-                 (forall C, classOf this σ1 C ->
-                       cname o1 <> C) ->
-                 exists χ ϕ ψ x y s C, reductions M σ1 (χ, ϕ :: ψ) /\
-                                  contn ϕ = c_stmt ((x ◌ f) ≔ (r_ y) ;; s) /\
-                                  ⌊ x ⌋ (χ, ϕ :: ψ) ≜ (v_addr α) /\
-                                  classOf this (χ, ϕ :: ψ) C /\
-                                  classOf x (χ, ϕ :: ψ) C /\
-                                  ⌊ y ⌋ (χ, ϕ :: ψ) ≜ v2.
+                  forall χ1 ϕ1 ψ1 χ2 ϕ2 ψ2,
+                    σ1 = (χ1, ϕ1 :: ψ1) ->
+                    σ2 = (χ2, ϕ2 :: ψ2) ->
+                    forall α o1 o2 f v1 v2,
+                      mapp σ1 α = Some o1 ->
+                      mapp σ2 α = Some o2 ->
+                      flds o1 f = Some v1 ->
+                      flds o2 f = Some v2 ->
+                      v1 <> v2 ->
+                      (forall C, classOf this σ1 C ->
+                                 cname o1 <> C) ->
+                      exists χ ϕ ψ x y s C, reductions M σ1 (χ, ϕ :: ψ) /\
+                                            contn ϕ = c_stmt ((x ◌ f) ≔ (r_ y) ;; s) /\
+                                            ⌊ x ⌋ (χ, ϕ :: ψ) ≜ (v_addr α) /\
+                                            classOf this (χ, ϕ :: ψ) C /\
+                                            classOf x (χ, ϕ :: ψ) C /\
+                                            ⌊ y ⌋ (χ, ϕ :: ψ) ≜ v2.
 Proof.
   intros.
   let χ := fresh "χ" in
@@ -1049,63 +1051,107 @@ Proof.
     crush.
 Qed.
 
-Definition is_internal (M1 M2 : mdl)(σ : config) :=
-  (exists α o CDef, mapp σ this = Some (v_addr α) /\
-               mapp σ α = Some o /\
-               M1 (cname o) = Some CDef).
+Definition is_internal (M1 M2 : mdl)(σ : config)(α : addr) :=
+  (exists o CDef, mapp σ α = Some o /\
+             M1 (cname o) = Some CDef).
 
-Definition is_external (M1 M2 : mdl)(σ : config) :=
-  (exists α o, mapp σ this = Some (v_addr α) /\
-          mapp σ α = Some o /\
-          M1 (cname o) = None).
+Definition is_external (M1 M2 : mdl)(σ : config)(α : addr) :=
+  (exists o, mapp σ α = Some o /\
+        M1 (cname o) = None).
+
+Definition is_internal_self (M1 M2 : mdl)(σ : config) :=
+  (exists α, mapp σ this = Some (v_addr α) /\
+        is_internal M1 M2 σ α).
+
+Definition is_external_self (M1 M2 : mdl)(σ : config) :=
+  (exists α, mapp σ this = Some (v_addr α) /\
+        is_external M1 M2 σ α).
+
+Lemma pair_reductions_is_external_1 :
+  forall M1 M2 σ1 σ2, M1 ⦂ M2 ⦿ σ1 ⤳⋆ σ2 ->
+                 is_external_self M1 M2 σ1.
+Proof.
+Admitted.
+
+Lemma pair_reductions_is_external_2 :
+  forall M1 M2 σ1 σ2, M1 ⦂ M2 ⦿ σ1 ⤳⋆ σ2 ->
+                 is_external_self M1 M2 σ2.
+Proof.
+Admitted.
 
 Lemma frame_arising_from_single_frame_external_internal_is_method_call_reductions :
   forall M σ1 σ2, reductions M σ1 σ2 ->
-             forall χ1 ϕ1,
-               σ1 = (χ1, ϕ1 :: nil) ->
-               forall M1 M2,
-                 M1 ⋄ M2 ≜ M ->
-                 is_external M1 M2 σ1 ->
-                 is_internal M1 M2 σ2 ->
-                 forall χ2 ϕ2 ψ2, σ2 = (χ2, ϕ2 :: ψ2) ->
-                             (exists α m β s, method_is_called σ1 α m β /\
-                                         contn ϕ2 = c_stmt s /\
-                                         stmt_in_method M χ1 α m s) \/
-                             (exists χ ϕ ψ α m β s, reductions M σ1 (χ, ϕ :: ψ) /\
-                                               method_is_called (χ, ϕ :: ψ) α m β /\
-                                               contn ϕ2 = c_stmt s /\
-                                               stmt_in_method M χ α m s).
+                  forall χ1 ϕ1,
+                    σ1 = (χ1, ϕ1 :: nil) ->
+                    forall M1 M2,
+                      M1 ⋄ M2 ≜ M ->
+                      is_external_self M1 M2 σ1 ->
+                      is_internal_self M1 M2 σ2 ->
+                      forall χ2 ϕ2 ψ2, σ2 = (χ2, ϕ2 :: ψ2) ->
+                                  (exists x α m β s, method_is_called σ1 x α m β /\
+                                                contn ϕ2 = c_stmt s /\
+                                                stmt_in_method M χ1 α m s) \/
+                                  (exists χ ϕ ψ x α m β s, reductions M σ1 (χ, ϕ :: ψ) /\
+                                                      method_is_called (χ, ϕ :: ψ) x α m β /\
+                                                      contn ϕ2 = c_stmt s /\
+                                                      stmt_in_method M χ α m s).
 Proof.
   intros.
   eapply frame_arising_from_single_frame_is_method_call_reductions;
     eauto.
-  unfold is_external, is_internal in *;
+  unfold is_external_self, is_external, is_internal_self, is_internal in *;
+    repeat destruct_exists_loo;
+    andDestruct;
     repeat destruct_exists_loo;
     andDestruct;
     subst;
     repeat map_rewrite.
   intros Hcontra;
     rewrite Hcontra in *.
-  rewrite Ha in Ha1;
-    inversion Ha1;
+  rewrite Ha0 in Ha;
+    inversion Ha;
     subst.
 
   let o' := fresh "o" in
   destruct (reductions_preserves_heap_locations_classes M (χ1, ϕ1::nil)(χ2, ϕ2 :: ψ2))
-    with (α:=α0)(o:=o0) as [o'];
+    with (α:=α)(o:=o0) as [o'];
     auto;
     andDestruct.
   repeat map_rewrite.
-  rewrite Ha0 in Ha3;
+  rewrite Ha1 in Ha3;
     inversion Ha3;
     subst.
-  rewrite Hb in *;
+  rewrite Hb1 in *;
+    crush.
+Qed.
+
+Lemma is_external_self_implies_not_is_internal :
+  forall M1 M2 σ, is_external_self M1 M2 σ ->
+                  ~ is_internal_self M1 M2 σ.
+Proof.
+  intros;
+    unfold is_internal_self, is_external_self, is_internal, is_external in *;
+    intro Hcontra;
+    repeat destruct_exists_loo;
+    andDestruct;
+    crush.
+Qed.
+
+Lemma is_internal_self_implies_not_is_external :
+  forall M1 M2 σ, is_internal_self M1 M2 σ ->
+                  ~ is_external_self M1 M2 σ.
+Proof.
+  intros;
+    intro Hcontra;
+    unfold is_internal_self, is_external_self, is_internal, is_external in *;
+    repeat destruct_exists_loo;
+    andDestruct;
     crush.
 Qed.
 
 Lemma is_external_implies_not_is_internal :
-  forall M1 M2 σ, is_external M1 M2 σ ->
-             ~ is_internal M1 M2 σ.
+  forall M1 M2 σ α, is_external M1 M2 σ α ->
+               ~ is_internal M1 M2 σ α.
 Proof.
   intros;
     unfold is_internal, is_external in *;
@@ -1116,22 +1162,22 @@ Proof.
 Qed.
 
 Lemma is_internal_implies_not_is_external :
-  forall M1 M2 σ, is_internal M1 M2 σ ->
-             ~ is_external M1 M2 σ.
+  forall M1 M2 σ α, is_internal M1 M2 σ α ->
+               ~ is_external M1 M2 σ α.
 Proof.
   intros;
     intro Hcontra;
-    unfold is_internal, is_external in *;
+    unfold is_internal_self, is_external_self, is_internal, is_external in *;
     repeat destruct_exists_loo;
     andDestruct;
     crush.
 Qed.
 
 Inductive stack_trace : mdl -> mdl -> config -> Prop :=
-| trace_initial : forall M1 M2 χ ϕ x s, is_external M1 M2 (χ, ϕ :: nil) ->
-                                   classOf this (χ, ϕ :: nil) ObjectName ->
-                                   contn ϕ = c_hole x s ->
-                                   stack_trace M1 M2 (χ, ϕ :: nil)
+| trace_initial : forall M1 M2 χ ϕ x s, is_external_self M1 M2 (χ, ϕ :: nil) ->
+                                        classOf this (χ, ϕ :: nil) ObjectName ->
+                                        contn ϕ = c_hole x s ->
+                                        stack_trace M1 M2 (χ, ϕ :: nil)
 | trace_internal : forall M1 M2 χ ϕ ψ x s C CDef m zs body,
     stack_trace M1 M2 (χ, ψ) ->
     contn ϕ = c_hole x s ->
@@ -1175,11 +1221,11 @@ Hint Constructors valid_stack_trace stack_trace : loo_db.
 
 Lemma valid_program_trace_reduction :
   forall M σ1 σ2, M ∙ σ1 ⤳ σ2 ->
-             forall M1 M2,
-               M_wf M1 ->
-               M1 ⋄ M2 ≜ M ->
-               valid_stack_trace M1 M2 σ1 ->
-               valid_stack_trace M1 M2 σ2.
+                  forall M1 M2,
+                    M_wf M1 ->
+                    M1 ⋄ M2 ≜ M ->
+                    valid_stack_trace M1 M2 σ1 ->
+                    valid_stack_trace M1 M2 σ2.
 Proof.
   intros M σ1 σ2 Hred;
     induction Hred;
@@ -1258,7 +1304,7 @@ Proof.
         eapply (ext_head M1 M2 χ) with (C:=C')(CDef:=CDef)(m:=m)(s:=s)(zs:=zs)(body:=body);
           eauto
       end;
-    
+      
       try solve [match goal with
                  | [Hcls : classOf _ _ _ |- _] =>
                    inversion Hcls;
@@ -1319,18 +1365,18 @@ Admitted.
 
 Lemma reduction_internal_external :
   forall M σ1 σ2, M ∙ σ1 ⤳ σ2 ->
-             M_wf M ->
-             forall χ1 ϕ1 ψ1 χ2 ϕ2 ψ2, σ1 = (χ1, ϕ1 :: ψ1) ->
-                                  σ2 = (χ2, ϕ2 :: ψ2) ->
-                                  forall M1 M2, M1 ⋄ M2 ≜ M ->
-                                           is_external M1 M2 σ1 ->
-                                           (is_external M1 M2 σ2 \/
-                                            (is_internal M1 M2 σ2 /\
-                                             exists C CDef m zs s s', classOf this σ2 C /\
-                                                                 M1 C = Some CDef /\
-                                                                 c_meths CDef m = Some (zs, s) /\
-                                                                 contn ϕ2 = c_stmt s' /\
-                                                                 substmt s' s)).
+                  M_wf M ->
+                  forall χ1 ϕ1 ψ1 χ2 ϕ2 ψ2, σ1 = (χ1, ϕ1 :: ψ1) ->
+                                            σ2 = (χ2, ϕ2 :: ψ2) ->
+                                            forall M1 M2, M1 ⋄ M2 ≜ M ->
+                                                          is_external_self M1 M2 σ1 ->
+                                                          (is_external_self M1 M2 σ2 \/
+                                                           (is_internal_self M1 M2 σ2 /\
+                                                            exists C CDef m zs s s', classOf this σ2 C /\
+                                                                                     M1 C = Some CDef /\
+                                                                                     c_meths CDef m = Some (zs, s) /\
+                                                                                     contn ϕ2 = c_stmt s' /\
+                                                                                     substmt s' s)).
 Proof.
   intros M σ1 σ2 Hred;
     induction Hred;
@@ -1386,15 +1432,724 @@ Proof.
       subst.*)
 
     
-      
+    
 Admitted.
+
+Definition meth_func :=
+  fun (M : mdl)(x : var)(α : addr)(m : mth)(β : partial_map var var)(σ : config) =>
+    let (χ, ψ) := σ in
+    match ψ with
+    | ϕ :: ψ' =>
+      let c := contn ϕ in
+      let β' := vMap ϕ in
+      match c with
+      | c_stmt (s_meth _ _ _ _ ;; s') =>
+        match χ α with
+        | Some o =>
+          match M (cname o) with
+          | Some CDef =>
+            match (c_meths CDef) m with
+            | Some (zs, body) =>
+              Some (χ, (frm (update this (v_addr α) (β ∘ β')) (c_stmt body))
+                         :: (frm β' (c_hole x s'))
+                         :: ψ')
+            | _ => None
+            end
+          | _ => None
+          end
+        | _ => None
+        end
+      | _ => None
+      end
+    | _ => None
+    end.
+
+Definition assgn_func :=
+  fun (x : var)(v : value)(σ : config) =>
+    let (χ, ψ) := σ in
+    match ψ with
+    | ϕ :: ψ' =>
+      let c := contn ϕ in
+      let β := vMap ϕ in
+      match c with
+      | c_stmt s =>
+        match s with
+        | s_asgn _ _ ;; s => Some (χ, (frm (update x v β) (c_stmt s)) :: ψ')
+        | _ => None
+        end
+      | _ => None
+      end
+    | _ => None
+    end.
+
+Definition new_func :=
+  fun (x : var)(o : obj)(α : addr)(σ : config) =>
+    let (χ, ψ) := σ in
+    match ψ with
+    | ϕ :: ψ' =>
+      let c := contn ϕ in
+      let β := vMap ϕ in
+      match c with
+      | c_stmt s =>
+        match s with
+        | s_new _ _ _ ;; s => Some (update α o χ, (frm (update x (v_addr α) β) (c_stmt s)) :: ψ')
+        | _ => None
+        end
+      | _ => None
+      end
+    | _ => None
+    end.
+
+Definition if_func : value -> config -> option config :=
+  fun (v : value)(σ : config) =>
+    let (χ, ψ) := σ in
+    match ψ with
+    | ϕ :: ψ' =>
+      let c := contn ϕ in
+      let β := vMap ϕ in
+      match c with
+      | c_stmt s =>
+        match s with
+        | s_if _ s1 s2 ;; s =>
+          match v with
+          | v_true => Some (χ, frm β (c_stmt (s1 ;; s)) :: ψ')
+          | v_false => Some (χ, frm β (c_stmt (s2 ;; s)) :: ψ')
+          | _ => None
+          end
+        | _ => None
+        end
+      | _ => None
+      end
+    | _ => None
+    end.
+
+Definition ret_func :=
+  fun (v : value)(σ : config) =>
+    let (χ, ψ) := σ in
+    match ψ with
+    | ϕ1 :: ϕ2 :: ψ' =>
+      let c1 := contn ϕ1 in
+      let c2 := contn ϕ2 in
+      let β := vMap ϕ2 in
+      match c2 with
+      | c_hole x s =>
+        match c1 with
+        | c_stmt (s_rtrn _) =>
+          Some (χ, frm (update x v β) (c_stmt s))
+        | c_stmt ((s_rtrn _) ;; _) =>
+          Some (χ, frm (update x v β) (c_stmt s))
+        | _ => None
+        end
+      | _ => None
+      end
+    | _ => None
+    end.
+
+
+Lemma reduction_function :
+  forall M σ1 σ2, M ∙ σ1 ⤳ σ2 ->
+                  exists f, f M σ1 = σ2.
+Proof.
+  intros M σ1 σ2 Hred;
+    induction Hred;
+    subst;
+    match goal with
+    | [|- exists f, f _ _ = ?σ] =>
+      exists (fun _ _ => σ)
+    end;
+    auto.
+
+Qed.
+
+
+
+Definition internal_obj (M1 M2 : mdl)(o : obj) : Prop :=
+  exists CDef, M1 (cname o) = CDef.
+
+Definition external_obj (M1 M2 : mdl)(o : obj) : Prop :=
+  exists CDef, M2 (cname o) = CDef.
+
+Definition internal_addr (M1 M2 : mdl)(σ : config)(α : addr) : Prop :=
+  exists o, mapp σ α = Some o ->
+            internal_obj M1 M2 o.
+
+Definition external_addr (M1 M2 : mdl)(σ : config)(α : addr) : Prop :=
+  exists o, mapp σ α = Some o ->
+            external_obj M1 M2 o.
+
+Definition no_external_calls (M1 M2 : mdl)(m : mth) : Prop :=
+  forall σ1 σ2, M1 ⦂ M2 ⦿ σ1 ⤳ σ2 ->
+                forall σ0 α1 α2  β, M1 ⦂ M2 ◎ σ0 … σ1 ⊨ (α1 calls α2 ▸ m ⟨ β ⟩) ->
+                                    exists χ1 ϕ1 ψ1 χ2 ϕ2 ψ2 s x y β',
+                                      σ1 = (χ1, ϕ1 :: ψ1) /\
+                                      σ2 = (χ2, ϕ2 :: ψ2) /\
+                                      length ψ1 = length ψ2 /\
+                                      vMap ϕ1 this = vMap ϕ2 this /\
+                                      contn ϕ1 = c_stmt (s_meth x y m β' ;; s) /\
+                                      contn ϕ2 = c_stmt s.
+
+Definition classic_spec (M1 M2 : mdl)(α1 α2 : addr)(m : mth)(β : partial_map var a_var)(A1 A2 : asrt) :=
+  forall σ1 σ2, M1 ⦂ M2 ⦿ σ1 ⤳ σ2 ->
+                (length (snd σ1)) = length (snd σ2) ->
+                forall σ0, M1 ⦂ M2 ◎ σ0 … σ1 ⊨ ((a_ α1) calls (a_ α2) ▸ m ⟨ β ⟩) ->
+                           M1 ⦂ M2 ◎ σ0 … σ1 ⊨ A1 ->
+                           M1 ⦂ M2 ◎ σ0 … σ2 ⊨ A2.
+
+Definition classic_spec_prop (M1 M2 : mdl)(C : cls)(m : mth)(P Q : mdl -> mdl -> config -> Prop) :=
+  forall σ1 σ2, M1 ⦂ M2 ⦿ σ1 ⤳ σ2 ->
+                (length (snd σ1)) = length (snd σ2) ->
+                (exists CDef body, M1 C = Some CDef /\
+                                   c_meths CDef m = body) ->
+                forall σ0 α1 α2 β o, M1 ⦂ M2 ◎ σ0 … σ1 ⊨ ((a_ α1) calls (a_ α2) ▸ m ⟨ β ⟩) ->
+                                     mapp σ1 α1 = Some o ->
+                                     cname o = C ->
+                                     P M1 M2 σ1 ->
+                                     Q M1 M2 σ2.
+
+Inductive reductions_alt : mdl -> mdl -> config -> config -> Prop :=
+| ra_single : forall M1 M2 M σ1 σ2, M1 ⋄ M2 ≜ M ->
+                                    M ∙ σ1 ⤳ σ2 ->
+                                    is_internal_self M1 M2 σ1 ->
+                                    is_external_self M1 M2 σ2 ->
+                                    reductions_alt M1 M2 σ1 σ2
+| ra_trans : forall M1 M2 M σ1 σ2 σ, M1 ⋄ M2 ≜ M ->
+                                     M ∙ σ1 ⤳ σ2 ->
+                                     is_internal_self M1 M2 σ1 ->
+                                     reductions_alt M1 M2 σ2 σ ->
+                                     reductions_alt M1 M2 σ1 σ.
+
+Inductive pair_reduction_alt : mdl -> mdl -> config -> config -> Prop :=
+| pra : forall M1 M2 M σ1 σ σ2, M1 ⋄ M2 ≜ M ->
+                           M ∙ σ1 ⤳ σ ->
+                           is_external_self M1 M2 σ1 ->
+                           reductions_alt M1 M2 σ σ2 ->
+                           pair_reduction_alt M1 M2 σ1 σ2.
+
+Inductive pair_reductions_alt : mdl -> mdl -> config -> config -> Prop :=
+| pra_single : forall M1 M2 σ1 σ2, pair_reduction_alt M1 M2 σ1 σ2 ->
+                              pair_reductions_alt M1 M2 σ1 σ2
+| pra_trans : forall M1 M2 σ1 σ σ2, pair_reduction_alt M1 M2 σ1 σ ->
+                               pair_reductions_alt M1 M2 σ σ2 ->
+                               pair_reductions_alt M1 M2 σ1 σ2.
+
+Hint Constructors pair_reductions_alt.
+
+Lemma reductions_step_e_assgn :
+  forall M1 M2 σ1 σ2, reductions_alt M1 M2 σ1 σ2 ->
+                      forall χ ϕ ψ M x e v s,
+                        σ1 = (χ, ϕ :: ψ) ->
+                        contn ϕ = c_stmt ((r_ x) ≔ (r_exp e) ;; s) ->
+                        M1 ⋄ M2 ≜ M ->
+                        M ∙ σ1 ⊢ e ↪ v ->
+                        exists σ, assgn_func x v σ1 = Some σ /\
+                                  M ∙ σ1 ⤳ σ /\
+                                  reductions_alt M1 M2 σ σ2.
+Proof.
+  intros M1 M2 σ1 σ2 Hred;
+    inversion Hred;
+    intros;
+    subst.
+
+  - match goal with
+    | [Ha : _ ∙ _ ⤳ _|- _] =>
+      inversion Ha;
+        subst;
+        try solve [crush]
+    end.
+    match goal with
+    | [Ha : contn ?ϕ = _,
+            Hb : contn ?ϕ = _ |- _] =>
+      rewrite Ha in Hb;
+        inversion Hb;
+        subst;
+        clear Hb
+    end.
+    match goal with
+    | [Ha : is_external_self _ _ _ |- _ ] =>
+      apply is_external_self_implies_not_is_internal in Ha;
+        contradiction Ha
+    end.
+    unfold is_internal_self, is_internal in *;
+      repeat destruct_exists_loo;
+      andDestruct;
+      repeat destruct_exists_loo;
+      andDestruct;
+      repeat map_rewrite.
+    unfold vMap in *.
+    repeat eq_auto.
+    repeat eexists; eauto.
+
+  - match goal with
+    | [Ha : _ ∙ _ ⤳ _|- _] =>
+      inversion Ha;
+        subst;
+        try solve [crush]
+    end.
+    match goal with
+    | [Ha : contn ?ϕ = _,
+            Hb : contn ?ϕ = _ |- _] =>
+      rewrite Ha in Hb;
+        inversion Hb;
+        subst;
+        clear Hb
+    end.
+    unfold assgn_func.
+    match goal with
+    | [Ha : contn ?ϕ = _ |- context [contn ?ϕ]] =>
+      rewrite Ha; simpl
+    end.
+    link_unique_auto.
+    eval_rewrite.
+    eexists;
+      repeat split;
+      eauto.
+Qed.
+
+Lemma reductions_step_assgn :
+  forall M1 M2 σ1 σ2, reductions_alt M1 M2 σ1 σ2 ->
+                      forall χ ϕ ψ M x e v s,
+                        σ1 = (χ, ϕ :: ψ) ->
+                        contn ϕ = c_stmt (((r_ x) ≔ (r_exp e)) ;; s) ->
+                        M1 ⋄ M2 ≜ M ->
+                        M ∙ σ1 ⊢ e ↪ v ->
+                        exists σ, assgn_func x v σ1 = Some σ /\
+                                  M ∙ σ1 ⤳ σ /\
+                                  reductions_alt M1 M2 σ σ2.
+Proof.
+  intros M1 M2 σ1 σ2 Hred;
+    inversion Hred;
+    intros;
+    subst.
+
+  - match goal with
+    | [Ha : _ ∙ _ ⤳ _|- _] =>
+      inversion Ha;
+        subst;
+        try solve [crush]
+    end.
+    match goal with
+    | [Ha : contn ?ϕ = _,
+            Hb : contn ?ϕ = _ |- _] =>
+      rewrite Ha in Hb;
+        inversion Hb;
+        subst;
+        clear Hb
+    end.
+    match goal with
+    | [Ha : is_external_self _ _ _ |- _ ] =>
+      apply is_external_self_implies_not_is_internal in Ha;
+        contradiction Ha
+    end.
+    unfold is_internal_self, is_internal in *;
+      repeat destruct_exists_loo;
+      andDestruct;
+      repeat destruct_exists_loo;
+      andDestruct;
+      repeat map_rewrite.
+    unfold vMap in *.
+    repeat eq_auto.
+    repeat eexists; eauto.
+
+  - match goal with
+    | [Ha : _ ∙ _ ⤳ _|- _] =>
+      inversion Ha;
+        subst;
+        try solve [crush]
+    end.
+    match goal with
+    | [Ha : contn ?ϕ = _,
+            Hb : contn ?ϕ = _ |- _] =>
+      rewrite Ha in Hb;
+        inversion Hb;
+        subst;
+        clear Hb
+    end.
+    unfold assgn_func.
+    match goal with
+    | [Ha : contn ?ϕ = _ |- context [contn ?ϕ]] =>
+      rewrite Ha; simpl
+    end.
+    link_unique_auto.
+    eval_rewrite.
+    eexists;
+      repeat split;
+      eauto.
+Qed.
+
+(*Lemma reductions_step_if :
+  forall M1 M2 σ1 σ2, reductions_alt M1 M2 σ1 σ2 ->
+                      forall χ ϕ ψ M e s1 s2 s,
+                        σ1 = (χ, ϕ :: ψ) ->
+                        contn ϕ = c_stmt ((s_if e s1 s2) ;; s) ->
+                        M1 ⋄ M2 ≜ M ->
+                        (exists σ, if_func v_true σ1 = Some σ /\
+                                   M ∙ σ1 ⤳ σ /\
+                                   reductions_alt M1 M2 σ σ2 /\
+                                   M ∙ σ1 ⊢ e ↪ v_true) \/
+                        (exists σ, if_func v_false σ1 = Some σ /\
+                                   M ∙ σ1 ⤳ σ /\
+                                   reductions_alt M1 M2 σ σ2 /\
+                                   M ∙ σ1 ⊢ e ↪ v_false).
+Proof.
+  intros M1 M2 σ1 σ2 Hred;
+    inversion Hred;
+    intros;
+    subst.
+
+  - match goal with
+    | [Ha : _ ∙ _ ⤳ _|- _] =>
+      inversion Ha;
+        subst;
+        try solve [crush]
+    end.
+    + match goal with
+      | [Ha : contn ?ϕ = _,
+              Hb : contn ?ϕ = _ |- _] =>
+        rewrite Ha in Hb;
+          inversion Hb;
+          subst;
+          clear Hb
+      end.
+      match goal with
+      | [Ha : is_external _ _ _ |- _ ] =>
+        apply is_external_implies_not_is_internal in Ha;
+          contradiction Ha
+      end.
+    + match goal with
+      | [Ha : contn ?ϕ = _,
+              Hb : contn ?ϕ = _ |- _] =>
+        rewrite Ha in Hb;
+          inversion Hb;
+          subst;
+          clear Hb
+      end.
+      match goal with
+      | [Ha : is_external _ _ _ |- _ ] =>
+        apply is_external_implies_not_is_internal in Ha;
+          contradiction Ha
+      end.
+
+  - match goal with
+    | [Ha : _ ∙ _ ⤳ _|- _] =>
+      inversion Ha;
+        subst;
+        try solve [crush]
+    end.
+    + match goal with
+      | [Ha : contn ?ϕ = _,
+              Hb : contn ?ϕ = _ |- _] =>
+        rewrite Ha in Hb;
+          inversion Hb;
+          subst;
+          clear Hb
+      end.
+      unfold if_func.
+      match goal with
+      | [Ha : contn ?ϕ = _ |- context [contn ?ϕ]] =>
+        rewrite Ha; simpl
+      end.
+      link_unique_auto.
+      left;
+        eexists;
+        repeat split;
+        eauto.
+    + match goal with
+      | [Ha : contn ?ϕ = _,
+              Hb : contn ?ϕ = _ |- _] =>
+        rewrite Ha in Hb;
+          inversion Hb;
+          subst;
+          clear Hb
+      end.
+      unfold if_func.
+      match goal with
+      | [Ha : contn ?ϕ = _ |- context [contn ?ϕ]] =>
+        rewrite Ha; simpl
+      end.
+      link_unique_auto.
+      eval_rewrite.
+      right;
+        eexists;
+        repeat split;
+        eauto.
+Qed.*)
+
+Lemma pair_reduction_change_alt :
+  forall M1 M2 σ1 σ2, pair_reductions_alt M1 M2 σ1 σ2 ->
+                 forall (P : mdl -> mdl -> config -> Prop),
+                   P M1 M2 σ1 ->
+                   ~ P M1 M2 σ2 ->
+                   exists σ σ', (σ = σ1 \/ pair_reductions_alt M1 M2 σ1 σ) /\
+                           pair_reduction_alt M1 M2 σ σ' /\
+                           (σ' = σ2 \/ pair_reductions_alt M1 M2 σ' σ2) /\
+                           P M1 M2 σ /\
+                           ~ P M1 M2 σ'.
+Proof.
+  intros M1 M2 σ1 σ2 Hred;
+    induction Hred;
+    intros;
+    auto with loo_db.
+
+  - exists σ1, σ2; repeat split;
+      auto.
+
+  - destruct (excluded_middle (P M1 M2 σ)).
+    + specialize (IHHred P);
+        repeat auto_specialize;
+        repeat destruct_exists_loo;
+        andDestruct.
+      exists σ0, σ3; repeat split; eauto.
+      right.
+      destruct Ha;
+        subst;
+        eauto.
+
+    + exists σ1, σ;
+        repeat split;
+        eauto.
+Qed.
+
+
+Lemma pair_reduction_alt_equiv_1 :
+  forall M1 M2 σ1 σ2, pair_reduction_alt M1 M2 σ1 σ2 ->
+                 M1 ⦂ M2 ⦿ σ1 ⤳ σ2.
+Proof.
+
+Admitted.
+
+Lemma pair_reductions_alt_equiv_1 :
+  forall M1 M2 σ1 σ2, pair_reductions_alt M1 M2 σ1 σ2 ->
+                 M1 ⦂ M2 ⦿ σ1 ⤳⋆ σ2.
+Proof.
+Admitted.
+
+
+Lemma pair_reduction_alt_equiv_2 :
+  forall M1 M2 σ1 σ2, M1 ⦂ M2 ⦿ σ1 ⤳ σ2 ->
+                 pair_reduction_alt M1 M2 σ1 σ2.
+Proof.
+
+Admitted.
+
+Lemma pair_reductions_alt_equiv_2 :
+  forall M1 M2 σ1 σ2, M1 ⦂ M2 ⦿ σ1 ⤳⋆ σ2 ->
+                 pair_reductions_alt M1 M2 σ1 σ2.
+Proof.
+Admitted.
+
+Lemma pair_reduction_change :
+  forall M1 M2 σ1 σ2, M1 ⦂ M2 ⦿ σ1 ⤳⋆ σ2 ->
+                 forall (P : mdl -> mdl -> config -> Prop),
+                   P M1 M2 σ1 ->
+                   ~ P M1 M2 σ2 ->
+                   exists σ σ', (σ = σ1 \/ M1 ⦂ M2 ⦿ σ1 ⤳⋆ σ) /\
+                           M1 ⦂ M2 ⦿ σ ⤳ σ' /\
+                           (σ' = σ2 \/ M1 ⦂ M2 ⦿ σ' ⤳⋆ σ2) /\
+                           P M1 M2 σ /\
+                           ~ P M1 M2 σ'.
+Proof.
+  intros.
+  destruct (pair_reduction_change_alt M1 M2 σ1 σ2)
+    with (P:=P)
+    as [σ];
+    auto.
+  apply pair_reductions_alt_equiv_2; auto.
+  repeat destruct_exists_loo;
+    andDestruct.
+  exists σ, σ0;
+    repeat split;
+    auto.
+  + destruct Ha; auto.
+    right; apply pair_reductions_alt_equiv_1; auto.
+  + apply pair_reduction_alt_equiv_1; auto.
+  + destruct Ha1; auto.
+    right; apply pair_reductions_alt_equiv_1; auto.
+Qed.
+
+Lemma asgn_reduction_step :
+  forall M σ1 σ2, M ∙ σ1 ⤳ σ2 ->
+                  forall χ ϕ ψ, σ1 = (χ, ϕ :: ψ) ->
+                                forall x r s, contn ϕ = c_stmt (((r_ x) ≔ r) ;; s) ->
+                                              exists v, σ2 = (χ, frm (update x v (vMap ϕ)) (c_stmt s) :: ψ) /\
+                                                        ((exists y, r = r_var y /\ vMap ϕ y = Some v) \/
+                                                         (exists e, r = r_exp e /\ M ∙ σ1 ⊢ e ↪ v)).
+Proof.
+
+Admitted.
+
+Lemma if_reduction_step :
+  forall M σ1 σ2, M ∙ σ1 ⤳ σ2 ->
+                  forall χ ϕ ψ, σ1 = (χ, ϕ :: ψ) ->
+                                forall e s1 s2 s, contn ϕ = c_stmt ((s_if e s1 s2) ;; s) ->
+                                                  (σ2 = (χ, frm (vMap ϕ) (c_stmt (s1 ;; s)) :: ψ) /\
+                                                   M ∙ σ1 ⊢ e ↪ v_true) \/
+                                                  (σ2 = (χ, frm (vMap ϕ) (c_stmt (s2 ;; s)) :: ψ) /\
+                                                   M ∙ σ1 ⊢ e ↪ v_false).
+Proof.
+
+Admitted.
+
+Lemma vAssgn_reductions_step :
+  forall M1 M2 σ1 σ2, reductions_alt M1 M2 σ1 σ2 ->
+                      forall M χ ϕ ψ, σ1 = (χ, ϕ :: ψ) ->
+                                      M1 ⋄ M2 ≜ M ->
+                                      forall x r s, contn ϕ = c_stmt (((r_ x) ≔ r) ;; s) ->
+                                                    exists σ v, σ = (χ, frm (update x v (vMap ϕ)) (c_stmt s) :: ψ) /\
+                                                                ((exists e, r = r_exp e /\
+                                                                            M ∙ σ1 ⊢ e ↪ v) \/
+                                                                 (exists y f α o, r = r_fld y f /\
+                                                                                  vMap ϕ y = Some (v_addr α) /\
+                                                                                  χ α = Some o /\
+                                                                                  flds o f = Some v)) /\
+                                                                reductions_alt M1 M2 σ σ2 /\
+                                                                M ∙ σ1 ⤳ σ /\
+                                                                is_internal_self M1 M2 σ1 /\
+                                                                is_internal_self M1 M2 σ.
+Proof.
+
+Admitted.
+
+Lemma fAssgn_reductions_step :
+  forall M1 M2 σ1 σ2, reductions_alt M1 M2 σ1 σ2 ->
+                      forall M χ ϕ ψ, σ1 = (χ, ϕ :: ψ) ->
+                                      M1 ⋄ M2 ≜ M ->
+                                      forall x f y s, contn ϕ = c_stmt ((x ◌ f ≔ (r_ y)) ;; s) ->
+                                                 exists σ v α o, σ = (update α (new (cname o) (update f v (flds o))) χ,
+                                                                 frm (vMap ϕ) (c_stmt s):: ψ) /\
+                                                            vMap ϕ y = Some v /\
+                                                            vMap ϕ x = Some (v_addr α) /\
+                                                            χ α = Some o /\
+                                                            (exists v', flds o f = Some v') /\
+                                                            reductions_alt M1 M2 σ σ2 /\
+                                                            M ∙ σ1 ⤳ σ /\
+                                                            is_internal_self M1 M2 σ1 /\
+                                                            is_internal_self M1 M2 σ.
+Proof.
+
+Admitted.
+
+Lemma if_reductions_step :
+  forall M1 M2 σ1 σ2, reductions_alt M1 M2 σ1 σ2 ->
+                      forall M χ ϕ ψ, σ1 = (χ, ϕ :: ψ) ->
+                                      M1 ⋄ M2 ≜ M ->
+                                      forall e s1 s2 s, contn ϕ = c_stmt ((s_if e s1 s2) ;; s) ->
+                                                        exists σ, ((σ = (χ, frm (vMap ϕ) (c_stmt (merge s1 s)) :: ψ) /\
+                                                                    M ∙ σ1 ⊢ e ↪ v_true) \/
+                                                                   (σ = (χ, frm (vMap ϕ) (c_stmt (merge s2 s)) :: ψ) /\
+                                                                    M ∙ σ1 ⊢ e ↪ v_false)) /\
+                                                                  reductions_alt M1 M2 σ σ2 /\
+                                                                  M ∙ σ1 ⤳ σ /\
+                                                                  is_internal_self M1 M2 σ1 /\
+                                                                  is_internal_self M1 M2 σ.
+Proof.
+
+Admitted.
+
+Lemma rtrn_1_reductions_step :
+  forall M1 M2 σ1 σ2, reductions_alt M1 M2 σ1 σ2 ->
+                 forall M χ ϕ1 ϕ2 ψ,
+                   σ1 = (χ, ϕ1 :: ϕ2 :: ψ) ->
+                   M1 ⋄ M2 ≜ M ->
+                   forall x1 s1 x2 s2, contn ϕ1 = c_stmt ((s_rtrn x1) ;; s1) ->
+                                  contn ϕ2 = c_hole x2 s2 ->
+                                  exists σ v, (σ = (χ, frm (update x2 v (vMap ϕ2)) (c_stmt s2) :: ψ)) /\
+                                         (vMap ϕ1 x1 = Some v) /\
+                                         (M ∙ σ1 ⤳ σ)  /\
+                                         ((reductions_alt M1 M2 σ σ2 /\
+                                           is_internal_self M1 M2 σ1 /\
+                                           is_internal_self M1 M2 σ) \/
+                                          (σ2 = σ /\
+                                           is_internal_self M1 M2 σ1 /\
+                                           is_external_self M1 M2 σ)).
+Proof.
+
+Admitted.
+
+Ltac reduction_step :=
+  match goal with
+
+    
+  | [H : reductions_alt ?M1 ?M2
+                        (?χ', {| vMap := ?β; contn := (c_stmt ((?x' ◌ ?f' ≔ (r_ ?y')) ;; ?s)) |} :: ?ψ')
+                        ?σ2,
+         Hlink : ?M1 ⋄ ?M2 ≜ ?M |- _ ] =>
+    let σ := fresh "σ" in
+    edestruct
+      (fAssgn_reductions_step
+         M1 M2
+         (χ', {| vMap := β; contn := (c_stmt ((x' ◌ f' ≔ (r_ y')) ;; s)) |} :: ψ')
+         σ2
+         H)
+      with
+        (ϕ:={| vMap := β; contn := (c_stmt ((x' ◌ f' ≔ (r_ y')) ;; s)) |})
+        (M:=M)(χ:=χ')(ψ:=ψ')
+      as [σ];
+    clear H
+
+    
+  | [H : reductions_alt ?M1 ?M2
+                        (?χ', {| vMap := ?β; contn := (c_stmt ((?y ≔ ?r') ;; ?s)) |} :: ?ψ')
+                        ?σ2,
+         Hlink : ?M1 ⋄ ?M2 ≜ ?M |- _ ] =>
+    let σ := fresh "σ" in
+    edestruct
+      (vAssgn_reductions_step
+         M1 M2
+         (χ', {| vMap := β; contn := (c_stmt ((y ≔ r') ;; s)) |} :: ψ')
+         σ2
+         H)
+      with
+        (ϕ:={| vMap := β; contn := (c_stmt ((y ≔ r') ;; s)) |})
+        (r:=r')(M:=M)(χ:=χ')(ψ:=ψ')
+      as [σ];
+    clear H
+
+          
+  | [H : reductions_alt ?M1 ?M2
+                        (?χ', {| vMap := ?β; contn := (c_stmt ((s_if ?e' ?s1' ?s2') ;; ?s')) |} :: ?ψ')
+                        ?σ2,
+         Hlink : ?M1 ⋄ ?M2 ≜ ?M |- _ ] =>
+    let σ := fresh "σ" in
+    edestruct
+      (if_reductions_step
+         M1 M2
+         (χ', {| vMap := β; contn := (c_stmt ((s_if e' s1' s2') ;; s')) |} :: ψ')
+         σ2
+         H)
+      with
+        (ϕ:={| vMap := β; contn := (c_stmt ((s_if e' s1' s2') ;; s')) |})
+        (e:=e')(s1:=s1')(s2:=s2')(M:=M)(χ:=χ')(ψ:=ψ')(s:=s')
+      as [σ];
+    clear H
+
+          
+  | [H : reductions_alt ?M1 ?M2
+                        (?χ', {| vMap := ?β1; contn := (c_stmt ((s_rtrn ?x1') ;; ?s1')) |}
+                                :: {| vMap := ?β2; contn := (c_hole ?x2' ?s2') |}
+                                :: ?ψ')
+                        ?σ2',
+         Hlink : ?M1 ⋄ ?M2 ≜ ?M |- _ ] => 
+    let σ := fresh "σ" in
+    edestruct (rtrn_1_reductions_step
+                 M1 M2
+                 (χ', {| vMap := β1; contn := (c_stmt ((s_rtrn x1') ;; s1')) |}
+                        :: {| vMap := β2; contn := (c_hole x2' s2') |}
+                        :: ψ')
+                 σ2'
+                 H)
+      with
+        (ϕ1:={| vMap := β1; contn := (c_stmt ((s_rtrn x1') ;; s1')) |})
+        (ϕ2:={| vMap := β2; contn := (c_hole x2' s2') |})
+      as [σ];
+    clear H
+  end.
 
 Module SafeExample.
 
-(**
+  (**
 ∀s.[s : Safe ∧ s.treasure <> null ∧ will(s.treasure = null) 
         ⟶ ∃o.[external(o) ∧ (o access s.secret)]]
- *)
+   *)
 
   (** Safe Definition *)
 
@@ -1406,17 +2161,19 @@ Module SafeExample.
 
   Definition take := methID 0.
 
-  Definition scr := bnd 0.
+  Definition scr := bnd 1.
 
-  Definition x := bnd 1.
+  Definition x := bnd 2.
 
-  Definition y := bnd 2.
+  Definition y := bnd 3.
 
-  Definition takeBody := ((r_ x) ≔ (r_exp (e_val (v_null))) ;;
-                         (s_if ((e_var scr) ⩵ (e_acc_f (e_var this) secret))
-                               ((r_ y) ≔ (this ◌ secret) ;; ((this ◌ secret) ≔ (r_ x)) ;; (s_rtrn y))
-                               (s_rtrn x)) ;;
-                         (s_rtrn x)).
+  Definition takeBody := ((r_ x) ≔ (r_exp (e_val (v_null)))) ;;
+                         (((r_ y) ≔ (this ◌ treasure)) ;;
+                          ((s_if ((e_var scr) ⩵ (e_acc_f (e_var this) secret))
+                                 (((this ◌ treasure) ≔ (r_ x)) ;;
+                                  (s_rtrn y))
+                                 (s_rtrn x)) ;;
+                           (s_rtrn x))).
 
   Definition SafeDef1 := clazz Safe
                                (treasure :: secret :: nil)
@@ -1429,20 +2186,643 @@ Module SafeExample.
 
   Definition MyModule1 := (update
                              Safe SafeDef1
-                             empty).    
+                             empty).
 
+  Lemma link_MyModule1_Safe :
+    forall M' M, MyModule1 ⋄ M' ≜ M ->
+            M Safe = Some SafeDef1.
+  Proof.
+    intros.
+    inversion H;
+      subst;
+      simpl.
+    unfold MyModule1, extend in *; simpl.
+    repeat map_rewrite.
+  Qed.
+
+
+
+  Lemma take_implies_secret :
+    forall M1 M2 σ1 σ2, pair_reduction_alt MyModule1 M2 σ1 σ2 ->
+                   M1 = MyModule1 ->
+                   forall x α β o, method_is_called σ1 x α take β ->
+                              mapp σ1 α = Some o ->
+                              cname o = Safe ->
+                              exists v, flds o secret = Some v.
+  Proof.
+    intros M1 M2 σ1 σ2 Hred;
+      inversion Hred;
+      subst;
+      intros.
+
+    inversion H4; subst.
+    inversion H0; subst;
+      repeat simpl_crush;
+      try solve [crush].
+    interpretation_rewrite.
+    simpl_crush.
+    unfold mapp, configMapHeap, fst in H5.
+    
+    match goal with
+    | [Ha : ?χ ?α = Some _,
+            Hb : ?χ ?α = Some _ |- _] =>
+      rewrite Ha in Hb;
+        inversion Hb;
+        subst
+    end.
+    match goal with
+    | [Ha : cname ?o = _,
+            Hb : context[cname ?o] |- _] =>
+      rewrite Ha in Hb
+    end.
+    erewrite link_MyModule1_Safe in H13;
+      eauto.
+    inversion H13;
+      subst.
+    simpl in H14.
+    unfold update, t_update in H14;
+      eq_auto.
+    inversion H14;
+      subst.
+    unfold takeBody in H2.
+
+    reduction_step;
+      simpl; eauto;
+        destruct_exists_loo;
+        andDestruct;
+        subst;
+        simpl in *.
+    destruct Ha0 as [|Htmp];
+      [|destruct Htmp];
+      repeat destruct_exists_loo;
+      andDestruct;
+      try solve [crush].
+
+    match goal with
+    | [H : r_exp _ = r_exp _ |- _] =>
+      inversion H; subst
+    end.
+
+    reduction_step;
+      simpl; eauto;
+        destruct_exists_loo;
+        andDestruct;
+        subst;
+        simpl in *.
+    destruct Ha1 as [|Htmp];
+      [|destruct Htmp];
+      repeat destruct_exists_loo;
+      andDestruct;
+      try solve [crush].
+
+    match goal with
+    | [H : (?x ◌ ?f) = (_ ◌ _) |- _] =>
+      inversion H; subst
+    end.
+
+    assert (α0=α);
+      [repeat map_rewrite;
+       unfold x, this;
+       crush
+      |subst α0].
+
+    reduction_step;
+      simpl; eauto;
+        andDestruct;
+        subst;
+        simpl in *;
+        andDestruct.
+    destruct Ha4;
+      andDestruct;
+      subst.
+
+    - match goal with
+      | [Heval : ?M ∙ ?σ ⊢ (_ ⩵ e_acc_f (e_var this) secret) ↪ ?v |- _] =>
+        inversion Heval;
+          subst
+      end.
+      match goal with
+      | [Heval : ?M ∙ ?σ ⊢ (e_acc_f (e_var this) secret) ↪ ?v |- _] =>
+        inversion Heval;
+          subst
+      end.
+      repeat map_rewrite.
+      match goal with
+      | [Heval : ?M ∙ ?σ ⊢ (e_var this) ↪ ?v |- _] =>
+        inversion Heval;
+          subst
+      end.
+      repeat map_rewrite.
+      simpl in *.
+      match goal with
+      | [H : Some _ = Some _ |- _]  =>
+        inversion H;
+          subst;
+          clear H
+      end.
+      repeat match goal with
+             | [Ha : ?m ?a = _, Hb : ?m ?a = _ |- _]  =>
+               rewrite Ha in Hb;
+                 inversion Hb;
+                 subst
+             end.
+      eauto.
+
+    - match goal with
+      | [Heval : ?M ∙ ?σ ⊢ (_ ⩵ e_acc_f (e_var this) secret) ↪ ?v |- _] =>
+        inversion Heval;
+          subst
+      end.
+      match goal with
+      | [Heval : ?M ∙ ?σ ⊢ (e_acc_f (e_var this) secret) ↪ ?v |- _] =>
+        inversion Heval;
+          subst
+      end.
+      repeat map_rewrite.
+      match goal with
+      | [Heval : ?M ∙ ?σ ⊢ (e_var this) ↪ ?v |- _] =>
+        inversion Heval;
+          subst
+      end.
+      repeat map_rewrite.
+      simpl in *.
+      match goal with
+      | [H : Some _ = Some _ |- _]  =>
+        inversion H;
+          subst;
+          clear H
+      end.
+      repeat match goal with
+             | [Ha : ?m ?a = _, Hb : ?m ?a = _ |- _]  =>
+               rewrite Ha in Hb;
+                 inversion Hb;
+                 subst
+             end.
+      eauto.
+
+  Qed.                            
+
+  Lemma take_implies_treasure :
+    forall M1 M2 σ1 σ2, pair_reduction_alt MyModule1 M2 σ1 σ2 ->
+                   M1 = MyModule1 ->
+                   forall x α β o, method_is_called σ1 x α take β ->
+                              mapp σ1 α = Some o ->
+                              cname o = Safe ->
+                              exists v, flds o treasure = Some v.
+  Proof.
+    intros M1 M2 σ1 σ2 Hred;
+      inversion Hred;
+      subst;
+      intros.
+
+    inversion H4; subst.
+    inversion H0; subst;
+      repeat simpl_crush;
+      try solve [crush].
+    interpretation_rewrite.
+    unfold mapp, configMapHeap, fst in H5.
+    repeat simpl_crush.
+    match goal with
+    | [Ha : cname ?o = _,
+            Hb : context[cname ?o] |- _] =>
+      rewrite Ha in Hb
+    end.
+    erewrite link_MyModule1_Safe in H13;
+      eauto.
+    inversion H13;
+      subst.
+    simpl in H14.
+    unfold update, t_update in H14;
+      eq_auto.
+    inversion H14;
+      subst.
+    unfold takeBody in H2.
+
+    reduction_step;
+      simpl; eauto;
+        repeat destruct_exists_loo;
+        andDestruct.
+    destruct Ha0 as [|Htmp];
+      [|destruct Htmp];
+      try solve [crush];
+      subst;
+      andDestruct;
+      simpl in *.
+
+    reduction_step;
+      simpl; eauto;
+        repeat destruct_exists_loo;
+        andDestruct.
+    destruct Ha0 as [|Htmp];
+      [|destruct Htmp];
+      try solve [crush];
+      subst;
+      andDestruct;
+      simpl in *.
+
+    repeat destruct_exists_loo;
+      andDestruct.
+    match goal with
+    | [H : _ ◌ _ = _ ◌ _  |- _] =>
+      inversion H; subst
+    end.
+    assert (this <> x);
+      [unfold this, x; crush|].
+    repeat map_rewrite;
+      repeat match goal with
+             | [H : Some _ = Some _ |- _] =>
+               inversion H; subst
+             end.
+    match goal with
+    | [Ha : ?m ?a = _, Hb : ?m ?a = _ |- _] =>
+      rewrite Ha in Hb;
+        inversion Hb;
+        subst;
+        clear Hb
+    end.
+    eauto.
+  Qed.
+
+  Lemma pair_reduction_take_is_called :
+    forall M σ1 σ2, MyModule1 ⦂ M ⦿ σ1 ⤳ σ2 ->
+               forall χ ϕ ψ,
+                 σ1 = (χ, ϕ :: ψ) ->
+                 exists x α β o, method_is_called σ1 x α take β /\
+                            mapp σ1 α = Some o /\
+                            cname o = Safe.
+  Proof.
+  Admitted.
+
+  Lemma take_pre_post_alt :
+    forall M1 M2 σ1 σ2, pair_reduction_alt M1 M2 σ1 σ2 ->
+                   M1 = MyModule1 ->
+                   forall χ ϕ ψ s1 s2,
+                     σ1 = (χ, ϕ :: ψ) ->
+                     contn ϕ = c_stmt (s1 ;; s2) ->
+                     forall x α β o, method_is_called σ1 x α take β ->
+                                mapp σ1 α = Some o ->
+                                cname o = Safe ->
+                                exists t s, flds o treasure = Some t /\
+                                       flds o secret = Some s /\
+                                       ((β scr = Some s /\
+                                         σ2 = (update α (new Safe (update treasure v_null (flds o))) χ,
+                                               (frm (update x t (vMap ϕ)) (c_stmt s2)) :: ψ)) \/
+                                        ((exists s', β scr = Some s' /\
+                                                s' <> s /\
+                                                σ2 = (χ,
+                                                      frm (update x v_null (vMap ϕ)) (c_stmt s2)
+                                                          :: ψ)))).
+  Proof.
+    intros M1 M2 σ1 σ2 Hred;
+      inversion Hred;
+      intros;
+      subst.
+
+    inversion H10; subst.
+    inversion H0; subst;
+      try simpl_crush;
+      try solve [crush].
+    match goal with
+    | [Ha : contn ?ϕ = _,
+            Hb : contn ?ϕ = _ |- _] =>
+      rewrite Ha in Hb;
+        inversion Hb;
+        subst
+    end.
+    interpretation_rewrite.
+    match goal with
+    | [Ha : (v_addr _) = (v_addr _) |- _] =>
+      inversion Ha;
+        subst
+    end.
+    assert (o0 = o);
+      [repeat map_rewrite; crush|subst].
+    match goal with
+    | [Ha : cname ?o = ?C',
+            Hb : ?M (cname ?o) = ?Def' |- _] =>
+      rewrite Ha in Hb
+    end.
+    assert (C = SafeDef1);
+    [apply linked_class with (C:=Safe)(Def:=SafeDef1) in H; auto;
+        [|unfold Safe, ObjectName; crush];
+        match goal with
+        | [Ha : ?m ?a = _, Hb : ?m ?a = _ |- _] =>
+          rewrite Ha in Hb;
+          inversion Hb;
+          subst;
+          clear Hb
+        end;
+        auto|subst].
+
+    match goal with
+    | [H : c_meths SafeDef1 take = Some (_, _) |- _] =>
+      unfold SafeDef1 in H;
+        simpl in H;
+        unfold update, t_update in H;
+        eq_auto;
+        inversion H;
+        subst;
+        clear H
+    end.
+    repeat simpl_crush.
+
+    match goal with
+    | [H : reductions_alt _ _ (_, {|vMap := _; contn := c_stmt takeBody |} :: _ :: _) _ |- _] =>
+      unfold takeBody in H
+    end.
+
+    reduction_step;
+      simpl; eauto;
+        repeat destruct_exists_loo;
+        andDestruct;
+        subst.
+    destruct Ha0 as [|Htmp];
+      [|destruct Htmp];
+      try solve [crush];
+      destruct_exists_loo;
+      andDestruct.
+    match goal with
+    | [H : r_exp _ = r_exp _ |- _] =>
+      inversion H;
+        subst;
+        clear H
+    end.
+    match goal with
+    | [H: _ ∙ _ ⊢ e_null ↪ ?v |- _] =>
+      inversion H;
+        subst
+    end.
+
+    reduction_step;
+      simpl; eauto;
+        repeat destruct_exists_loo;
+        andDestruct;
+        subst.
+    destruct Ha0 as [|Htmp];
+      [|destruct Htmp];
+      try solve [crush];
+      repeat destruct_exists_loo;
+      andDestruct;
+      simpl in *.
+    assert (this <> x);
+      [unfold x, this;
+       crush|].
+    repeat simpl_crush.
+    assert (α0 = α);
+      [repeat map_rewrite;
+       repeat eq_auto;
+       repeat simpl_crush;
+       auto|subst; simpl_crush].
+
+    exists v.
+
+    reduction_step;
+      simpl; eauto;
+        andDestruct;
+        subst.
+    destruct Ha;
+      andDestruct;
+      subst.
+
+    - (*scr == secret*)
+      assert (exists s, flds o0 secret = Some s /\ (ps ∘ (vMap ϕ0)) scr = Some s).
+      + match goal with
+        | [Heval : _ ∙ _ ⊢ (_ ⩵ (e_acc_f (e_var this) secret)) ↪ v_true |- _] =>
+          inversion Heval;
+            subst
+        end.
+        match goal with
+        | [Heval : _ ∙ _ ⊢ (e_acc_f (e_var this) secret) ↪ ?v |- _] =>
+          inversion Heval;
+            subst
+        end.
+        match goal with
+        | [Heval : _ ∙ _ ⊢ ((e_var this)) ↪ ?v |- _] =>
+          inversion Heval;
+            subst
+        end.
+        repeat map_rewrite.
+        simpl in *.
+        repeat simpl_crush.
+        exists v0; split; auto.
+        match goal with
+        | [Heval : _ ∙ _ ⊢ (e_var scr) ↪ ?v |- _ = Some ?v] =>
+          inversion Heval; subst
+        end.
+        unfold mapp, configMapStack, mapp, stackMap, snd, vMap in H14.
+        simpl in H14.
+        auto.
+
+      + destruct_exists_loo; andDestruct.
+        exists v0; repeat split; auto.
+        left; split; auto.
+        simpl in *.
+
+        reduction_step;
+          simpl; eauto;
+            repeat destruct_exists_loo;
+            andDestruct;
+            subst;
+            simpl in *.
+        assert (x <> y);
+          [unfold y, x; crush|].
+        unfold update, t_update in Ha8;
+          repeat eq_auto;
+          repeat simpl_crush.
+
+        unfold mapp, configMapHeap, fst in H11.
+        assert (y <> this);
+          [unfold y, this; crush|].
+        unfold update, t_update in Ha9;
+          repeat eq_auto;
+          repeat simpl_crush.
+
+        repeat match goal with
+               | [Ha : ?P, Hb : ?P |-_] =>
+                 clear Hb
+               end.
+
+        reduction_step;
+          simpl; eauto;
+            repeat destruct_exists_loo
+            repeat simpl_crush;
+            andDestruct;
+            subst;
+            simpl in *;
+            repeat destruct_exists_loo;
+            andDestruct.
+        destruct Hb1;
+          andDestruct;
+          subst.
+        * apply is_internal_self_implies_not_is_external in Hb4.
+          contradiction Hb4.
+          unfold is_external_self, is_external.
+          unfold is_external_self, is_external in H1;
+            repeat destruct_exists_loo;
+            andDestruct;
+            repeat destruct_exists_loo;
+            andDestruct.
+          exists α; split; [|exists o0];
+          unfold mapp, configMapStack, configMapHeap, mapp, snd, fst, stackMap;
+            simpl;
+            [|split; auto].
+          unfold update, t_update;
+            eq_auto.
+          assert (α <> α0);
+            [|unfold update, t_update; eq_auto].
+          intros Hcontra;
+            subst.
+          unfold mapp, configMapHeap, fst in Ha9.
+          repeat simpl_crush.
+          match goal with
+          | [H : cname ?o = Safe |- _] =>
+            rewrite H in *
+          end.
+          repeat simpl_crush.
+          match goal with
+          | [H : MyModule1 Safe = None |- _] =>
+            unfold MyModule1 in H;
+              simpl in H;
+              unfold update, t_update in H;
+              repeat eq_auto
+          end.
+          crush.
+
+        * assert (x <> y);
+            [unfold x, y; crush|].
+          unfold update, t_update in Ha3;
+            repeat eq_auto;
+            repeat simpl_crush.
+          match goal with
+          | [H : cname ?o = Safe |- context[cname ?o]] =>
+            rewrite H
+          end.
+          auto.
+
+    - (*scr ⩵̸ secret*)
+      simpl in *.
+      assert (exists s s', flds o0 secret = Some s /\ (ps ∘ (vMap ϕ0)) scr = Some s' /\ s <> s').
+      + match goal with
+        | [Heval : _ ∙ _ ⊢ (_ ⩵ (e_acc_f (e_var this) secret)) ↪ v_false |- _] =>
+          inversion Heval;
+            subst
+        end.
+        match goal with
+        | [Heval : _ ∙ _ ⊢ (e_acc_f (e_var this) secret) ↪ ?v |- _] =>
+          inversion Heval;
+            subst
+        end.
+        match goal with
+        | [Heval : _ ∙ _ ⊢ ((e_var this)) ↪ ?v |- _] =>
+          inversion Heval;
+            subst
+        end.
+        repeat map_rewrite.
+        simpl in *.
+        repeat simpl_crush.
+        match goal with
+        | [Heval : _ ∙ _ ⊢ (e_var scr) ↪ ?v |- _] =>
+          inversion Heval; subst
+        end.
+        unfold mapp, configMapStack, mapp, stackMap, snd, vMap in H18.
+        simpl in H18.
+        exists v2, v1; split; auto.
+
+      + repeat destruct_exists_loo; andDestruct.
+        exists v0; repeat split; auto.
+        right; exists v1; repeat split; auto.
+
+        reduction_step;
+          simpl; eauto;
+            repeat destruct_exists_loo;
+            andDestruct;
+            subst;
+            simpl in *.
+        assert (x <> y);
+          [unfold y, x; crush|].
+        unfold update, t_update in Ha9;
+          repeat eq_auto;
+          repeat simpl_crush.
+
+        repeat match goal with
+               | [Ha : ?P, Hb : ?P |-_] =>
+                 clear Hb
+               end.
+
+(*        unfold mapp, configMapHeap, fst in H12.
+        assert (y <> this);
+          [unfold y, this; crush|].
+        unfold update, t_update in Ha10;
+          repeat eq_auto;
+          repeat simpl_crush.
+
+        repeat match goal with
+               | [Ha : ?P, Hb : ?P |-_] =>
+                 clear Hb
+               end.*)
+
+        destruct Hb5;
+          andDestruct;
+          subst;
+          auto.
+        apply is_internal_self_implies_not_is_external in Hb1.
+        contradiction Hb1.
+        unfold is_external_self, is_external.
+        unfold is_external_self, is_external in H1;
+          repeat destruct_exists_loo;
+          andDestruct;
+          repeat destruct_exists_loo;
+          andDestruct.
+        exists α0; split; [|exists o];
+          unfold mapp, configMapStack, configMapHeap, mapp, snd, fst, stackMap;
+          simpl;
+          repeat split;
+          auto.
+        unfold update, t_update;
+          eq_auto;
+          auto.
+  Qed.
+
+  Lemma take_pre_post :
+    forall M σ1 σ2, MyModule1 ⦂ M ⦿ σ1 ⤳ σ2 ->
+               forall χ ϕ ψ s1 s2,
+                 σ1 = (χ, ϕ :: ψ) ->
+                 contn ϕ = c_stmt (s1 ;; s2) ->
+                 forall x α β o, method_is_called σ1 x α take β ->
+                            mapp σ1 α = Some o ->
+                            cname o = Safe ->
+                            exists t s, flds o treasure = Some t /\
+                                   flds o secret = Some s /\
+                                   ((β scr = Some s /\
+                                     σ2 = (update α (new Safe (update treasure v_null (flds o))) χ,
+                                           (frm (update x t (vMap ϕ)) (c_stmt s2)) :: ψ)) \/
+                                    ((exists s', β scr = Some s' /\
+                                            s' <> s /\
+                                            σ2 = (χ,
+                                                  frm (update x v_null (vMap ϕ)) (c_stmt s2)
+                                                      :: ψ)))).
+  Proof.
+    intros.
+    eapply take_pre_post_alt; eauto.
+    eapply pair_reduction_alt_equiv_2; eauto.
+  Qed.                   
+  
   Definition HolisticSpec := (∀x∙ (∀x∙(((a_class (a♢1) Safe)
                                         ∧
                                         ((ex_acc_f (e♢1) secret) ⩶ (e♢0))
                                         ∧
                                         ((ex_acc_f (e♢1) treasure) ⩶̸ (ex_null))
-                                        ∧
-                                        (a_will (((ex_acc_f (e♢1) treasure) ⩶ (ex_null)))))
-                                         ⟶
-                                         (∃x∙ (((a♢0) external)
-                                               ∧
-                                               ((a♢0) access (a♢1))))
-                             ))).
+                                         ∧
+                                         (a_will ((ex_acc_f (e♢1) treasure) ⩶ (ex_null))))
+                                           ⟶
+                                           (a_will (∃x∙ (((a♢0) external)
+                                                         ∧
+                                                         ((a♢0) access (a♢1))))
+                                            ∨
+                                            (∃x∙ (((a♢0) external)
+                                                  ∧
+                                                  ((a♢0) access (a♢1))))
+                             )))).
 
   Theorem safe_example :
     MyModule1 ⊨m HolisticSpec.
@@ -1455,17 +2835,104 @@ Module SafeExample.
     a_prop.
     inversion H5;
       subst.
+    let σ := fresh "σ" in
+    destruct (pair_reduction_change MyModule1 M' (χ, ϕ :: nil) σ')
+      with (P := fun (M1 M2 : mdl)(σ : config) =>
+                   M1 ⦂ M2 ◎ (χ, ϕ :: nil) … σ ⊨ (ex_acc_f (e_ α) treasure ⩶̸ (ex_null)))
+      as [σ];
+      auto.
+    + eapply sat_head_exp; eauto.
+      eapply sat_initial_exp; eauto.
 
-    let χ := fresh "χ" in
-    let ψ := fresh "ψ" in
-    destruct σ' as [χ ψ].
+    + intros Hcontra.
+      inversion H15; subst.
+      inversion Hcontra;
+        subst.
+      link_unique_auto.
+      repeat match goal with
+             | [H : is_exp ?e ?e' |- _] =>
+               inversion H;
+                 subst;
+                 clear H
+             end.
+      inversion H20; subst.
+      inversion H18; subst.
+      eval_rewrite.
+      crush.
 
-    assert (exists ϕ' ψ', ψ0 = ϕ' :: ψ');
-      [admit|repeat destruct_exists_loo; subst].
-    (*destruct (reductions_field_change M (χ, ϕ :: nil) (χ0, ϕ0 :: ψ1))
-      with (χ1:=χ)(ϕ1:=ϕ)(ψ2:=ψ1)(χ2:=χ0)(ϕ2:=ϕ0)(f:=treasure).*)
-              
+    + destruct_exists_loo;
+        andDestruct.
+      destruct Ha; subst.
+
+      * let x := fresh "x" in
+        destruct (pair_reduction_take_is_called M' (χ, ϕ :: nil) σ1)
+          with (χ0:=χ)(ϕ0:=ϕ)(ψ:=@nil frame)
+          as [x];
+          auto;
+          repeat destruct_exists_loo;
+          andDestruct.
+        inversion Ha;
+          subst.
+        let v := fresh "v" in
+        destruct (take_pre_post M' (χ, ϕ :: nil) σ1)
+          with (χ0:=χ)(ϕ0:=ϕ)(ψ:=@nil frame)(x:=x0)(α:=α1)(β:=β0 ∘ vMap ϕ)(o:=o1)
+               (s1:=s_meth x0 y0 take β0)(s2:=s)
+          as [v];
+          auto;
+          repeat destruct_exists_loo;
+          andDestruct.
+        inversion H7; subst.
+        repeat match goal with
+               | [H : is_exp _ _ |- _] =>
+                 inversion H;
+                   subst;
+                   clear H
+               end.
+        assert (α1 = α);
+          [admit|subst]. (* because α is the one that changes *)
+        assert (o1 = o);
+          [repeat map_rewrite; crush|subst].
+        inversion H19; subst.
+        inversion H14; subst.
+        inversion H16; subst.
+        inversion H12; subst.
+        assert (o1 = o);
+          [repeat map_rewrite; crush|subst].
+        assert (v0 = (v_addr α0));
+          [crush|subst].
+        destruct Hb2;
+          andDestruct;
+          subst.
+        ** assert (is_external_self MyModule1 M' (χ, ϕ :: ψ));
+             [apply pair_reductions_is_external_2 with (σ1:=σ0); auto|].
+           unfold is_external_self, is_external in H8;
+             repeat destruct_exists_loo;
+             andDestruct;
+             repeat destruct_exists_loo;
+             andDestruct.
+           link_unique_auto.
+
+           right.
+           apply sat_ex_x with (α:=α)(o:=o1);
+             simpl;
+             auto;
+             a_prop.
+           eapply sat_extrn; eauto.
+           unfold bind in Ha6; simpl in Ha6.
+           let x := fresh "x" in
+           destruct (partial_map_dec scr β0) as [x|Hnone];
+             [destruct_exists_loo|rewrite Hnone in Ha6; inversion Ha6].
+           eapply sat_access3 with (x:=x1); eauto.
+           eapply int_x; simpl; eauto.
+           eapply int_x; simpl; eauto.
+           rewrite H8 in Ha6; auto.
+           apply in_stmts_1.
+           apply in_meth_3.
+           exists scr; auto.
+
+        ** admit. (* contradiction: nothing changes, i.e. treasure <> null *)
+
+      * admit. (* above but again *)        
   Admitted.
 
 End SafeExample.
-
